backend/CSEproof.v
@@ -19,9 +19,6 @@ Require Import Op Registers RTL.
 Require Import ValueDomain ValueAOp ValueAnalysis.
 Require Import CSEdomain CombineOp CombineOpproof CSE.
 
-Section WITHROMEMFOR.
-Context `{romem_for_instance: ROMemFor}.
-
 Definition match_prog (prog tprog: RTL.program) :=
   match_program (fun cu f tf => transf_fundef (romem_for cu) f = OK tf) eq prog tprog.
 
@@ -30,8 +27,6 @@ Lemma transf_program_match:
 Proof.
   intros. eapply match_transform_partial_program_contextual; eauto.
 Qed.
-
-End WITHROMEMFOR.
 
 (** * Soundness of operations over value numberings *)
 
@@ -817,13 +812,9 @@ Section PRESERVATION.
 
 Variable prog: program.
 Variable tprog : program.
+Hypothesis TRANSF: match_prog prog tprog.
 Let ge := Genv.globalenv prog.
 Let tge := Genv.globalenv tprog.
-
-Section WITHROMEMFOR.
-Context `{romem_for_instance: ROMemFor}.
-
-Hypothesis TRANSF: match_prog prog tprog.
 
 Lemma symbols_preserved:
   forall (s: ident), Genv.find_symbol tge s = Genv.find_symbol ge s.
@@ -832,12 +823,6 @@ Proof (Genv.find_symbol_match TRANSF).
 Lemma senv_preserved:
   Senv.equiv ge tge.
 Proof (Genv.senv_match TRANSF).
-
-Lemma genv_next_preserved:
-  Genv.genv_next tge = Genv.genv_next ge.
-Proof.
-  apply senv_preserved.
-Qed.
 
 Lemma functions_translated:
   forall (v: val) (f: RTL.fundef),
@@ -897,25 +882,20 @@ Proof.
 Qed.
 
 Lemma find_function_translated:
-  forall ros rs fb fd rs',
-  find_block ge ros rs = Some fb ->
-  Genv.find_funct_ptr ge fb = Some fd ->
+  forall ros rs fd rs',
+  find_function ge ros rs = Some fd ->
   regs_lessdef rs rs' ->
-  exists cu tfb tfd, find_block tge ros rs' = Some tfb
-              /\ Genv.find_funct_ptr tge tfb = Some tfd
+  exists cu tfd, find_function tge ros rs' = Some tfd
               /\ transf_fundef (romem_for cu) fd = OK tfd
               /\ linkorder cu prog.
 Proof.
-  unfold find_block; intros; destruct ros.
-- specialize (H1 r). inv H1.
-  exploit funct_ptr_translated; eauto.
-  intros (cu & tf & FIND & TR & LINK); eauto.
-  exists cu, fb, tf; eauto.
-  rewrite <- H3 in H; discriminate.
-- rewrite symbols_preserved.
-  exploit funct_ptr_translated; eauto.
-  intros (cu & tf & FIND & TR & LINK); eauto.
-  exists cu, fb, tf; eauto.
+  unfold find_function; intros; destruct ros.
+- specialize (H0 r). inv H0.
+  apply functions_translated; auto.
+  rewrite <- H2 in H; discriminate.
+- rewrite symbols_preserved. destruct (Genv.find_symbol ge i).
+  apply funct_ptr_translated; auto.
+  discriminate.
 Qed.
 
 (** The proof of semantic preservation is a simulation argument using
@@ -963,16 +943,14 @@ Inductive match_states: state -> state -> Prop :=
       match_states (State s f sp pc rs m)
                    (State s' (transf_function' f approx) sp pc rs' m')
   | match_states_call:
-      forall s f tf args m s' args' m' cu b tb
-             (FIND: Genv.find_funct_ptr ge b = Some f)
-             (TFIND: Genv.find_funct_ptr tge tb = Some tf)
+      forall s f tf args m s' args' m' cu
              (LINK: linkorder cu prog)
              (STACKS: match_stackframes s s')
              (TFD: transf_fundef (romem_for cu) f = OK tf)
              (ARGS: Val.lessdef_list args args')
              (MEXT: Mem.extends m m'),
-      match_states (Callstate s b args m)
-                   (Callstate s' tb args' m')
+      match_states (Callstate s f args m)
+                   (Callstate s' tf args' m')
   | match_states_return:
       forall s s' v v' m m'
              (STACK: match_stackframes s s')
@@ -996,11 +974,9 @@ Ltac TransfInstr :=
 Lemma transf_step_correct:
   forall s1 t s2, step ge s1 t s2 ->
   forall s1' (MS: match_states s1 s1') (SOUND: sound_state prog s1),
-  exists w, (exists t', match_events_query _ w t t') /\
-  forall t', match_events cc_extends w t t' ->
-  exists s2', step tge s1' t' s2' /\ match_states s2 s2'.
+  exists s2', step tge s1' t s2' /\ match_states s2 s2'.
 Proof.
-  induction 1; intros; inv MS; try stable_step; try (TransfInstr; intro C).
+  induction 1; intros; inv MS; try (TransfInstr; intro C).
 
   (* Inop *)
 - econstructor; split.
@@ -1111,7 +1087,7 @@ Proof.
   eapply kill_loads_after_store_holds; eauto.
 
 - (* Icall *)
-  exploit find_function_translated; eauto. intros (cu' & tb & tf & FB' & FIND' & TRANSF' & LINK').
+  exploit find_function_translated; eauto. intros (cu' & tf & FIND' & TRANSF' & LINK').
   econstructor; split.
   eapply exec_Icall; eauto.
   eapply sig_preserved; eauto.
@@ -1123,7 +1099,7 @@ Proof.
   apply regs_lessdef_regs; auto.
 
 - (* Itailcall *)
-  exploit find_function_translated; eauto. intros (cu' & tb & tf & FB' & FIND' & TRANSF' & LINK').
+  exploit find_function_translated; eauto. intros (cu' & tf & FIND' & TRANSF' & LINK').
   exploit Mem.free_parallel_extends; eauto. intros [m'' [A B]].
   econstructor; split.
   eapply exec_Itailcall; eauto.
@@ -1135,9 +1111,7 @@ Proof.
   exploit (@eval_builtin_args_lessdef _ ge (fun r => rs#r) (fun r => rs'#r)); eauto.
   intros (vargs' & A & B).
   exploit external_call_mem_extends; eauto.
-  intros (w & Hwq & Hw). exists w; split; eauto.
-  intros t' Ht'. specialize (Hw t' Ht').
-  destruct Hw as (v' & m1' & P & Q & R & S).
+  intros (v' & m1' & P & Q & R & S).
   econstructor; split.
   eapply exec_Ibuiltin; eauto.
   eapply eval_builtin_args_preserved with (ge1 := ge); eauto. exact symbols_preserved.
@@ -1166,9 +1140,9 @@ Proof.
     exists valu.
     apply set_res_unknown_holds.
     InvSoundState. unfold vanalyze; rewrite AN.
-    assert (pmatch bc bsrc osrc (aaddr_arg (VA.State ae am) x1))
+    assert (pmatch bc bsrc osrc (aaddr_arg (VA.State ae am) a0))
     by (eapply aaddr_arg_sound_1; eauto).
-    assert (pmatch bc bdst odst (aaddr_arg (VA.State ae am) x))
+    assert (pmatch bc bdst odst (aaddr_arg (VA.State ae am) a1))
     by (eapply aaddr_arg_sound_1; eauto).
     eapply add_memcpy_holds; eauto.
     eapply kill_loads_after_storebytes_holds; eauto.
@@ -1211,7 +1185,6 @@ Proof.
   destruct or; simpl; auto.
 
 - (* internal function *)
-  rewrite FIND in H; inv H.
   monadInv TFD. unfold transf_function in EQ. fold (analyze cu f) in EQ.
   destruct (analyze cu f) as [approx|] eqn:?; inv EQ.
   exploit Mem.alloc_extends; eauto. apply Z.le_refl. apply Z.le_refl.
@@ -1223,12 +1196,9 @@ Proof.
   apply init_regs_lessdef; auto.
 
 - (* external function *)
-  rewrite FIND in H; inv H.
   monadInv TFD.
   exploit external_call_mem_extends; eauto.
-  intros (w & Hwq & Hw). exists w; split; eauto.
-  intros t' Ht'. specialize (Hw t' Ht').
-  destruct Hw as (v' & m1' & P & Q & R & S).
+  intros (v' & m1' & P & Q & R & S).
   econstructor; split.
   eapply exec_function_external; eauto.
   eapply external_call_symbols_preserved; eauto. apply senv_preserved.
@@ -1242,28 +1212,20 @@ Proof.
   apply set_reg_lessdef; auto.
 Qed.
 
-End WITHROMEMFOR.
-
-(* Whole-program case *)
-Local Existing Instance romem_for_wp_instance.
-
-Hypothesis TRANSF: match_prog prog tprog.
-
 Lemma transf_initial_states:
   forall st1, initial_state prog st1 ->
   exists st2, initial_state tprog st2 /\ match_states st1 st2.
 Proof.
   intros. inversion H.
   exploit funct_ptr_translated; eauto. intros (cu & tf & A & B & C).
-  exists (Callstate nil b nil m0); split.
+  exists (Callstate nil tf nil m0); split.
   econstructor; eauto.
   eapply (Genv.init_mem_match TRANSF); eauto.
   replace (prog_main tprog) with (prog_main prog).
   rewrite symbols_preserved. eauto.
-  assumption.
   symmetry. eapply match_program_main; eauto.
   rewrite <- H3. eapply sig_preserved; eauto.
-  econstructor; eauto. constructor. apply Mem.extends_refl.
+  econstructor. eauto. constructor. auto. auto. apply Mem.extends_refl.
 Qed.
 
 Lemma transf_final_states:
@@ -1274,19 +1236,16 @@ Proof.
 Qed.
 
 Theorem transf_program_correct:
-  forward_simulation cc_extends (RTL.semantics prog) (RTL.semantics tprog).
+  forward_simulation (RTL.semantics prog) (RTL.semantics tprog).
 Proof.
   eapply forward_simulation_step with
     (match_states := fun s1 s2 => sound_state prog s1 /\ match_states s1 s2).
 - apply senv_preserved.
-  assumption.
 - intros. exploit transf_initial_states; eauto. intros [s2 [A B]].
   exists s2. split. auto. split. apply sound_initial; auto. auto.
 - intros. destruct H. eapply transf_final_states; eauto.
 - intros. destruct H0. exploit transf_step_correct; eauto.
-  intros (w & Hwq & Hw). exists w; split; eauto.
-  intros t' Ht'. specialize (Hw t' Ht').
-  destruct Hw as [s2' [A B]]. exists s2'; split. auto. split. eapply sound_step; eauto. auto.
+  intros [s2' [A B]]. exists s2'; split. auto. split. eapply sound_step; eauto. auto.
 Qed.
 
 End PRESERVATION.
